wip

clightdm/mem/ClightDmMem1.v
@@ -21,7 +21,7 @@ Inductive tag :=
 | Local
 | Unfreeable.
 
-Record metadata := { blk : option block; sz : Z ; SZPOS: blk <> None -> sz > 0 }.
+Record metadata := { blk : option block; sz : Z ; SZPOS: sz >= 0 }.
 
 Let _pointstoRA: URA.t := (block ==> Z ==> (Consent.t memval))%ra.
 Let _allocatedRA: URA.t := (block ==> (Consent.t tag))%ra.
@@ -149,9 +149,7 @@ Section PROP.
 
   Definition m_null : metadata.
   Proof.
-    eapply Build_metadata.
-    instantiate (1:=0).
-    instantiate (1:=None). ss.
+    eapply Build_metadata. eapply None. instantiate (1:=0). lia.
   Defined.
 
   Definition disjoint (m m0: metadata) : Prop :=
@@ -993,7 +991,7 @@ Section SPEC.
   Definition salloc_spec: fspec :=
     (mk_simple (fun n => (
                     (ord_pure 0%nat),
-                    (fun varg => ⌜varg = n↑ /\ n ≤ Ptrofs.max_unsigned⌝),
+                    (fun varg => ⌜varg = n↑ /\ n ≤ Ptrofs.max_unsigned /\ n >= 0⌝),
                     (fun vret => ∃ m vaddr b,
                                  ⌜vret = b↑ /\ m.(blk) = Some b /\ m.(sz) = n ⌝
                                  ** vaddr (↦_m,1) List.repeat Undef (Z.to_nat n)
